code/mpfr/MPFR.Add1sp1.fst
@@ -28,7 +28,7 @@ module U32 = FStar.UInt32
 
 (* implementations *)
 (* intermediate results *)
-private type mpfr_tmp_exp_t = x:mpfr_exp_t{I64.(x >=^ mpfr_EMIN /\ x <=^ mpfr_EMAX +^ 1L)}
+private type mpfr_tmp_exp_t = x:mpfr_exp_t{I64.((*x >=^ mpfr_EMIN /\*) x <=^ mpfr_EMAX +^ 1L)} (*WARNING*)
 
 noeq type state = {
     sh:mpfr_reg_prec_t;
@@ -343,17 +343,13 @@ let mpfr_add1sp1 a b c rnd_mode p =
         let t = mpfr_add1sp1_round a ap rnd_mode st in
 	let h2 = ST.get() in
         assert(   as_val h1 (as_struct h1 a).mpfr_d * pow2 (as_normal_ h1 ({as_struct h1 a with mpfr_exp = st.bx})).len =(as_normal_ h1 ({as_struct h1 a with mpfr_exp = st.bx})).limb * pow2 64);
-        (* TO CLEAN*)
-        (  let aa=a in   let high=(as_normal_ h1 ({as_struct h1 a with mpfr_exp = st.bx})) in
-        let a=(add1sp_exact (as_reg_fp h0 b) (as_reg_fp h0 c)) in
-        lemma_pow2_mul (a.len-high.len) high.len;
-        assert(
-           high.limb * pow2 (a.len-high.len) = (high_mant a (I64.v (as_struct h0 aa).mpfr_prec)).limb);
-          assert(
-           high.limb * pow2 (a.len-high.len)*pow2 high.len = (high_mant a (I64.v (as_struct h0 aa).mpfr_prec)).limb*pow2 high.len);
-           lemma_paren_mul_right high.limb  (pow2 (a.len-high.len)) (pow2 high.len);
-          assert( high.limb *( pow2 (a.len-high.len)*pow2 high.len) = (high_mant a (I64.v (as_struct h0 aa).mpfr_prec)).limb*pow2 high.len);
-           lemma_pow2_mul (a.len-high.len) high.len );
+
+        (   let high=(as_normal_ h1 ({as_struct h1 a with mpfr_exp = st.bx})) in
+        let r=(add1sp_exact (as_reg_fp h0 b) (as_reg_fp h0 c)) in
+        lemma_pow2_mul (r.len-high.len) high.len;
+        assert(high.limb * pow2 (r.len-high.len)*pow2 high.len = (high_mant r (I64.v (as_struct h0 a).mpfr_prec)).limb*pow2 high.len); //
+        lemma_paren_mul_right high.limb  (pow2 (r.len-high.len)) (pow2 high.len);
+        lemma_pow2_mul (r.len-high.len) high.len );
            
 	mpfr_add1sp1_round_post_cond_lemma (add1sp_exact (as_reg_fp h0 b) (as_reg_fp h0 c)) (I64.v (as_struct h0 a).mpfr_prec) (as_normal_ h1 ({as_struct h1 a with mpfr_exp = st.bx})) (st.rb <> 0uL) (st.sb <> 0uL) rnd_mode (I32.v t) (as_fp h2 a); 
 	mpfr_modifies_trans_lemma a h0 h1 h2;
